working on return

src/lifting.v
@@ -37,11 +37,10 @@ Fixpoint no_return (s:stmt) :=
   | _ => True
   end.
   
-Definition wp_pre (wp : coPset -d> stmt -d> (option val → assert) -d> assert) :
-    coPset -d> stmt -d> (option val → assert) -d> assert := λ E s Q,
-  ((⌜s = skip⌝ ∧ |={E}=> Q None) ∨
+Definition wp_pre (wp : coPset -d> stmt -d> assert -d> assert) :
+    coPset -d> stmt -d> assert -d> assert := λ E s Q,
+  ((⌜s = skip⌝ ∧ |={E}=> Q) ∨
    (∀ σ ρ, ⎡state_interp σ ρ⎤ ={E,∅}=∗ ∀ r k, stack_match ρ r k -∗
-    (⌜k=[] -> no_return s⌝) -∗
     ∃ s' r' σ' k',
         ⌜step F s (Build_state r σ k) s' (Build_state r' σ' k')⌝ ∗
         ▷ |={∅,E}=> ∃ ρ', ⎡state_interp σ' ρ' ∗ (stack_match ρ' r' k' ∗ wp E s' Q) (stack_depth k')⎤))%I.
@@ -49,7 +48,7 @@ Definition wp_pre (wp : coPset -d> stmt -d> (option val → assert) -d> assert) 
 Local Instance wp_contractive : Contractive (wp_pre).
 Proof.
   rewrite /wp_pre /= => n wp wp' Hwp E s Q.
-  do 30 (f_contractive || f_equiv). apply Hwp.
+  do 29 (f_contractive || f_equiv). apply Hwp.
 Qed.
 
 Local Definition wp_def := fixpoint wp_pre.
@@ -61,10 +60,13 @@ Proof. rewrite -wp_aux.(seal_eq) //. Qed.
 Lemma wp_unfold E s Q : wp E s Q ⊣⊢ wp_pre wp E s Q.
 Proof. rewrite wp_unseal. apply (fixpoint_unfold wp_pre). Qed.
 
-Lemma wp_skip E Q : Q None ⊢ wp E skip Q.
+Definition wp' E s Q := (∀ R, <obj> (∀ e, (wp_expr E e (λ v, Q (Some v)) -∗ wp E (Sreturn e) R)) -∗
+  wp E s R)%I.
+
+Lemma wp_skip E Q : Q None ⊢ wp' E skip Q.
 Proof.
-  rewrite wp_unfold /wp_pre. iIntros. iLeft. iSplit; done.
-Qed.
+  rewrite /wp'. iIntros "? % He". admit.
+Admitted.
 
 Lemma var_e : forall x v σ ρ r k,
   stack_match ρ r k ∗ x ↦v v ∗ ⎡state_interp σ ρ⎤ ⊢ ⌜r !! x = Some v⌝.
@@ -123,49 +125,22 @@ Definition stack_retainer f := assert_of (λ n,
 Definition stackframe f vs := ([∗ list] x;v ∈ (get_params f ++ get_locals f);vs, points_to_var x v)%I.
 
 Definition call_assert E f vs x R := (⇑ (stack_retainer f -∗ stackframe f vs -∗
-  wp E (get_body f) ((λ v', ∃ v, ⌜Some v = v'⌝ ∧ stack_retainer f ∗
+  wp' E (get_body f) ((λ v', ∃ v, ⌜Some v = v'⌝ ∧ stack_retainer f ∗
     (∃ vs, ⌜stack_size f = length vs⌝ ∧ stackframe f vs) ∗
     ⇓ ((∃ v, points_to_var x v) ∗ ▷ (points_to_var x v -∗ R))))))%I.
 
 
-Lemma wp_return E e Q : wp_expr E e (λ v, Q $ Some v) ⊢ wp E (Sreturn e) Q.
+Lemma wp_return E e Q : wp_expr E e (λ v, Q $ Some v) ⊢ wp' E (Sreturn e) Q.
 Proof.
-  rewrite !wp_unfold /wp_pre.
-  iIntros "H".
-  iRight.
-  iIntros (σ ρ) "S".
-  rewrite /wp_expr.
-  iMod ("H" with "[$]") as "(% & He & ? & ?)".
-  iApply fupd_mask_intro; first set_solver.
-  iIntros "Hclose" (r k) "s %".
-  iDestruct ("He" with "[s]") as "%".
-  { by iApply stack_env_match. }
-
-  destruct k as [|(?, ?) ?].
-  { specialize (H eq_refl). rewrite /no_return // in H. }
-  iExists skip, _, σ, _.
-  iSplit.
-  { iPureIntro; by econstructor. }
-  iModIntro.
-  iMod "Hclose". iModIntro.
-  iExists _. iFrame.
-  iClear "Hclose".
-  iStopProof.
-  split => ?.
-  monPred.unseal. simpl.
-  rewrite /stack_match /stack_depth /=.
-  destruct (make_stack k) as [le depth] eqn:?.
-  rewrite !monPred_at_sep /stack_level /=.
-  monPred.unseal.
-  iIntros "(? & <- & ?)".
-  rewrite -wp_skip.
-Admitted.
+  iIntros "H % Hret". rewrite monPred_objectively_elim; by iApply "Hret".
+Qed.
 
 
 Lemma wp_assign E x e Q : wp_expr E e (λ v, (∃ v0, x ↦v v0) ∗
-  ▷ (x ↦v v -∗ Q None)) ⊢ wp E (Sassign x e) Q.
+  ▷ (x ↦v v -∗ Q None)) ⊢ wp' E (Sassign x e) Q.
 Proof.
-  rewrite wp_unfold /wp_pre /stack_depth. iIntros "H". iRight.
+  iIntros "H % Hret".
+  rewrite wp_unfold /wp_pre /stack_depth. iRight.
   iIntros (??) "S".
   rewrite /wp_expr.
   iMod ("H" with "S") as (?) "(He & S & (% & Hx) & Hpost)".
@@ -179,10 +154,11 @@ Proof.
   iMod "Hclose"; iModIntro.
   simpl.
   iApply (stack_match_embed with "[$]").
-  rewrite -wp_skip; by iApply "Hpost".
+  iApply (wp_skip with "[-Hret]"); last done.
+  by iApply "Hpost".
 Qed.
 
-Lemma wp_alloc E x Q : (∃ v0, x ↦v v0) ∗
+(*Lemma wp_alloc E x Q : (∃ v0, x ↦v v0) ∗
   ▷ (∀ l, points_to_var x (LocV l) -∗ l ↦ NumV 0 -∗ Q None) ⊢ wp E (Salloc x) Q.
 Proof.
   rewrite wp_unfold /wp_pre. iIntros "H". iRight.
@@ -220,16 +196,18 @@ Proof.
   iMod "Hclose"; iModIntro.
   iApply (stack_match_embed with "[$]").
   rewrite -wp_skip. by iApply "Hpost".
-Qed.
+Qed.*)
 
-Lemma wp_seq E s1 s2 Q : wp E s1 (λ _, ▷ wp E s2 Q) ⊢ wp E (Sseq s1 s2) Q.
+Lemma wp_seq E s1 s2 Q : wp E s1 (▷ wp' E s2 Q) ⊢ wp' E (Sseq s1 s2) Q.
 Proof.
+  iIntros "H % Hret".
+  rewrite {1}/wp'; iStopProof.
   split => i.
   iIntros "H".
   iLöb as "IH" forall (s1 s2 Q i).
   rewrite wp_unfold [wp _ (s1;;s2)%S _]wp_unfold /wp_pre.
-  (* set (wp as IH. *)
   monPred.unseal.
+  iDestruct "H" as "(H & Hret)".
   iRight.
   iIntros (???<-) "S".
   iDestruct "H" as "[[-> >Hs1] | H]".
@@ -239,6 +217,7 @@ Proof.
     { iNext; iFrame.
       destruct (make_stack x2).
       iMod "Hclose". iModIntro.
+      iSpecialize ("Hs1" with "[//] Hret").
       rewrite -monPred_at_sep.
       iApply (stack_match_stack_depth with "[$] [$]").
     }
@@ -252,7 +231,7 @@ Proof.
     iNext; iMod "H" as (ρ) "($ & ? & ?)"; iModIntro.
     rewrite -monPred_at_sep.
     iApply (stack_match_stack_depth with "[$] [-]").
-    iApply ("IH" with "[$]").
+    iApply "IH"; iFrame.
 Qed.
 
 Lemma wp_if E e s1 s2 Q : wp_expr E e (λ v, ∃ n, ⌜v = NumV n⌝ ∧
